ScalarMult: Z -> G -> G (closes #193)

src/Algebra/ScalarMult.v
@@ -1,91 +1,167 @@
+Require Import Coq.ZArith.BinInt Coq.omega.Omega Crypto.Util.ZUtil.Peano.
 Require Import Coq.Classes.Morphisms.
-Require Import Crypto.Algebra.Hierarchy Crypto.Algebra.Monoid.
-
-Module Import ModuloCoq8485.
-  Import NPeano Nat.
-  Infix "mod" := modulo.
-End ModuloCoq8485.
+Require Import Crypto.Util.Tactics.BreakMatch.
+Require Import Crypto.Algebra.Hierarchy Crypto.Algebra.Group.
+Local Open Scope Z_scope.
 
 Section ScalarMultProperties.
-  Context {G eq add zero} `{monoidG:@monoid G eq add zero}.
-  Context {mul:nat->G->G}.
+  Context {G eq add zero opp} `{groupG:@group G eq add zero opp}.
+  Context {mul:Z->G->G}.
   Local Infix "=" := eq : type_scope. Local Infix "=" := eq.
   Local Infix "+" := add. Local Infix "*" := mul.
   Class is_scalarmult :=
     {
       scalarmult_0_l : forall P, 0 * P = zero;
-      scalarmult_S_l : forall n P, S n * P = P + n * P;
+      scalarmult_succ_l_nn : forall n P, 0 <= n -> Z.succ n * P = P + n * P;
+      scalarmult_pred_l_np : forall n P, n <= 0 -> Z.pred n * P = opp P + n * P;
 
       scalarmult_Proper : Proper (Logic.eq==>eq==>eq) mul
     }.
   Global Existing Instance scalarmult_Proper.
   Context `{mul_is_scalarmult:is_scalarmult}.
 
-  Fixpoint scalarmult_ref (n:nat) (P:G) {struct n} :=
-    match n with
-    | O => zero
-    | S n' => add P (scalarmult_ref n' P)
-    end.
+  Lemma scalarmult_succ_l n P : Z.succ n * P = P + n * P.
+  Proof.
+    induction n using Z.peano_rect_strong; intros; rewrite ?Z.succ'_succ, ?Z.pred'_pred in * by omega;
+      repeat (rewrite ?scalarmult_0_l, ?scalarmult_succ_l_nn, ?scalarmult_pred_l_np, ?left_identity, ?right_identity, ?Z.succ_pred, ?Z.pred_succ, ?associative, ?right_inverse, ?left_inverse by omega); reflexivity.
+  Qed.
+
+  Lemma scalarmult_pred_l n P : Z.pred n * P = opp P + n * P.
+    induction n using Z.peano_rect_strong; intros; rewrite ?Z.succ'_succ, ?Z.pred'_pred in * by omega;
+      repeat (rewrite ?scalarmult_0_l, ?scalarmult_succ_l_nn, ?scalarmult_pred_l_np, ?left_identity, ?right_identity, ?Z.succ_pred, ?Z.pred_succ, ?associative, ?right_inverse, ?left_inverse by omega); reflexivity.
+  Qed.
+
+  Definition scalarmult_ref (n:Z) (P:G) : G :=
+    Z.peano_rect
+      (fun _ => G)
+      (zero)
+      (fun _ => add P)
+      (fun _ => add (opp P))
+      n
+  .
 
   Global Instance Proper_scalarmult_ref : Proper (Logic.eq==>eq==>eq) scalarmult_ref.
-  Proof using monoidG.
-    repeat intro; subst.
-    match goal with [n:nat |- _ ] => induction n; simpl @scalarmult_ref; [reflexivity|] end.
-    repeat match goal with [H:_ |- _ ] => rewrite H end; reflexivity.
+  Proof using groupG.
+    intros n n' H; subst n';
+      induction n using Z.peano_rect_strong;
+      cbv [Proper respectful] in *;
+      intros;
+      cbv [scalarmult_ref] in *; break_match; try reflexivity;
+      rewrite ?Z.peano_rect_succ, ?Z.peano_rect_pred in * by omega;
+      rewrite IHn by eassumption;
+      match goal with H : _ = _ |- _ => rewrite H; reflexivity end.
   Qed.
 
-  Lemma scalarmult_ext : forall n P, mul n P = scalarmult_ref n P.
+  Lemma scalarmult_ext n P : mul n P = scalarmult_ref n P.
   Proof using Type*.
-    induction n as [|n IHn]; simpl @scalarmult_ref; intros; rewrite <-?IHn; (apply scalarmult_0_l || apply scalarmult_S_l).
+    revert P.
+    destruct mul_is_scalarmult.
+    induction n using Z.peano_rect_strong; intros;
+      cbv [scalarmult_ref] in *; break_match;
+        rewrite ?Z.peano_rect_succ, ?Z.peano_rect_pred, ?Z.succ'_succ, ?Z.pred'_pred in *;
+        try rewrite <-IHn; try match goal with [H:_|-_] => eapply H end; omega.
   Qed.
 
-  Lemma scalarmult_1_l : forall P, 1*P = P.
-  Proof using Type*. intros. rewrite scalarmult_S_l, scalarmult_0_l, right_identity; reflexivity. Qed.
-
-  Lemma scalarmult_add_l : forall (n m:nat) (P:G), ((n + m)%nat * P = n * P + m * P).
+  Lemma scalarmult_1_l P : 1*P = P.
   Proof using Type*.
-    induction n as [|n IHn]; intros;
-      rewrite ?scalarmult_0_l, ?scalarmult_S_l, ?plus_Sn_m, ?plus_O_n, ?scalarmult_S_l, ?left_identity, <-?associative, <-?IHn; reflexivity.
+    intros. change 1 with (Z.succ 0).
+    rewrite scalarmult_succ_l, scalarmult_0_l, right_identity; reflexivity.
   Qed.
 
-  Lemma scalarmult_zero_r : forall m, m * zero = zero.
-  Proof using Type*. induction m as [|? IHm]; rewrite ?scalarmult_S_l, ?scalarmult_0_l, ?left_identity, ?IHm; try reflexivity. Qed.
+  Lemma scalarmult_opp1_l P : -1*P = opp P.
+    change (-1) with (Z.pred 0).
+    rewrite scalarmult_pred_l, scalarmult_0_l, right_identity; reflexivity.
+  Qed.
 
-  Lemma scalarmult_assoc : forall (n m : nat) P, n * (m * P) = (m * n)%nat * P.
+  Lemma scalarmult_add_l (n m:Z) (P:G) : ((n + m)%Z * P = n * P + m * P).
   Proof using Type*.
-    induction n as [|n IHn]; intros.
-    { rewrite <-mult_n_O, !scalarmult_0_l. reflexivity. }
-    { rewrite scalarmult_S_l, <-mult_n_Sm, <-Plus.plus_comm, scalarmult_add_l.
-      rewrite IHn. reflexivity. }
+    revert P.
+    induction n using Z.peano_rect_strong; intros; rewrite ?Z.succ'_succ, ?Z.pred'_pred in * by omega;
+        rewrite ?Z.add_0_l, ?Z.add_succ_l, ?Z.add_pred_l;
+        rewrite ?scalarmult_0_l, ?scalarmult_succ_l, ?scalarmult_pred_l, ?left_identity, <-?associative, <-?IHn; try reflexivity.
+  Qed.
+
+  Lemma scalarmult_opp_l (n:Z) (P:G) : (-n) * P = opp (n*P).
+  Proof using Type*.
+    revert P.
+    induction n using Z.peano_rect_strong; intros; rewrite ?Z.succ'_succ, ?Z.pred'_pred in * by omega.
+    { change (-0) with (0). rewrite !scalarmult_0_l, inv_id; reflexivity. }
+    { rewrite scalarmult_succ_l_nn, inv_op, <-IHn by omega.
+      replace (-Z.succ n) with (-n + (- 1))%Z by auto with zarith.
+      rewrite scalarmult_add_l, scalarmult_opp1_l; reflexivity. }
+    { rewrite scalarmult_pred_l_np, inv_op, <-IHn, inv_inv by omega.
+      replace (- Z.pred n) with (-n+1)%Z by auto with zarith.
+      rewrite scalarmult_add_l, scalarmult_1_l; reflexivity. }
+  Qed.
+
+  Lemma scalarmult_zero_r (n:Z) : n * zero = zero.
+    induction n using Z.peano_rect_strong; intros; rewrite ?Z.succ'_succ, ?Z.pred'_pred in * by omega;
+        rewrite ?scalarmult_0_l, ?scalarmult_succ_l_nn, ?scalarmult_pred_l_np, ?IHn, ?inv_id, ?left_identity by omega;
+        try reflexivity.
+  Qed.
+
+  Lemma scalarmult_assoc (n m : Z) P : n * (m * P) = (m * n)%Z * P.
+  Proof using Type*.
+    revert P.
+    induction n using Z.peano_rect_strong; intros; rewrite ?Z.succ'_succ, ?Z.pred'_pred in * by omega.
+    { rewrite Z.mul_0_r, 2scalarmult_0_l by omega; reflexivity. }
+    { rewrite scalarmult_succ_l, IHn by omega.
+      rewrite (Z.mul_comm m (Z.succ n)), Z.mul_succ_l, (Z.mul_comm n m), (Z.add_comm (m*n) m).
+      rewrite scalarmult_add_l. reflexivity. }
+    { rewrite scalarmult_pred_l, IHn by omega.
+      rewrite (Z.mul_comm m (Z.pred n)), Z.mul_pred_l, (Z.mul_comm n m), <-Z.add_opp_l.
+      rewrite scalarmult_add_l, scalarmult_opp_l. reflexivity. }
+  Qed.
+
+  Lemma scalarmult_sub_l (a b:Z) (P:G) : (a - b)*P = a*P + opp(b*P).
+  Proof using Type*.
+    rewrite <-Z.add_opp_r, scalarmult_add_l, scalarmult_opp_l; reflexivity.
+  Qed.
+
+  Lemma scalarmult_opp_r (n:Z) (P:G) : n*opp P = opp (n * P).
+  Proof using Type*.
+    revert P.
+    induction n using Z.peano_rect_strong; intros; rewrite ?Z.succ'_succ, ?Z.pred'_pred in * by omega;
+      rewrite <-?Z.add_1_l, <-?Z.sub_1_r;
+      [|rewrite Z.add_comm at 1|rewrite <-Z.add_opp_l; rewrite Z.add_comm at 1];
+      repeat (rewrite ?scalarmult_0_l, ?scalarmult_opp_l, ?scalarmult_add_l, ?inv_id, ?inv_op, ?inv_inv, ?IHn, ?scalarmult_1_l);
+      reflexivity.
   Qed.
 
   Lemma scalarmult_times_order : forall l B, l*B = zero -> forall n, (l * n) * B = zero.
   Proof using Type*. intros ? ? Hl ?. rewrite <-scalarmult_assoc, Hl, scalarmult_zero_r. reflexivity. Qed.
 
-  Lemma scalarmult_mod_order : forall l B, l <> 0%nat -> l*B = zero -> forall n, n mod l * B = n * B.
+  Lemma scalarmult_mod_order : forall l B, l <> 0 -> l*B = zero -> forall n, n mod l * B = n * B.
   Proof using Type*.
     intros l B Hnz Hmod n.
-    rewrite (NPeano.Nat.div_mod n l Hnz) at 2.
+    rewrite (Z.div_mod n l Hnz) at 2.
     rewrite scalarmult_add_l, scalarmult_times_order, left_identity by auto. reflexivity.
   Qed.
+
 End ScalarMultProperties.
 
 Section ScalarMultHomomorphism.
-  Context {G EQ ADD ZERO} {monoidG:@monoid G EQ ADD ZERO}.
-  Context {H eq add zero} {monoidH:@monoid H eq add zero}.
+  Context {G EQ ADD ZERO OPP} {groupG:@group G EQ ADD ZERO OPP}.
+  Context {H eq add zero opp} {groupH:@group H eq add zero opp}.
   Local Infix "=" := eq : type_scope. Local Infix "=" := eq : eq_scope.
-  Context {MUL} {MUL_is_scalarmult:@is_scalarmult G EQ ADD ZERO MUL }.
-  Context {mul} {mul_is_scalarmult:@is_scalarmult H eq add zero mul }.
+  Context {MUL} {MUL_is_scalarmult:@is_scalarmult G EQ ADD ZERO OPP MUL}.
+  Context {mul} {mul_is_scalarmult:@is_scalarmult H eq add zero opp mul}.
   Context {phi} {homom:@Monoid.is_homomorphism G EQ ADD H eq add phi}.
-  Context (phi_ZERO:phi ZERO = zero).
 
   Lemma homomorphism_scalarmult : forall n P, phi (MUL n P) = mul n (phi P).
   Proof using Type*.
-    setoid_rewrite scalarmult_ext.
-    induction n as [|n IHn]; intros; simpl; rewrite ?Monoid.homomorphism, ?IHn; easy.
+    induction n using Z.peano_rect_strong; intros; rewrite ?Z.succ'_succ, ?Z.pred'_pred in * by omega;
+      rewrite ?scalarmult_0_l, ?scalarmult_succ_l, ?scalarmult_pred_l by omega.
+    { apply homomorphism_id. }
+    { rewrite <-IHn. rewrite Monoid.homomorphism. reflexivity. }
+    { rewrite <-IHn. rewrite Monoid.homomorphism, Group.homomorphism_inv. reflexivity. }
   Qed.
 End ScalarMultHomomorphism.
 
-Global Instance scalarmult_ref_is_scalarmult {G eq add zero} `{@monoid G eq add zero}
-  : @is_scalarmult G eq add zero (@scalarmult_ref G add zero).
-Proof. split; try exact _; intros; reflexivity. Qed.
+Global Instance scalarmult_ref_is_scalarmult {G eq add zero opp} {groupG:@group G eq add zero opp}
+  : @is_scalarmult G eq add zero opp (@scalarmult_ref G add zero opp).
+Proof.
+  split; try exact _; cbv [scalarmult_ref] in *; intros;
+    rewrite <-?Z.succ'_succ, <-?Z.pred'_pred, ?Z.peano_rect_succ, ?Z.peano_rect_pred in * by omega;
+    reflexivity.
+Qed.
